discharge mem expr to z3 v1

extracted_code/EqCheck.ml
@@ -3,8 +3,8 @@ open Sexplib
 let equivalence_check_programs str1 str2 =
   let sexp_1 = Sexp.of_string str1 in
   let sexp_2 = Sexp.of_string str2 in
-  let prog_1 = Interface.coq_CaracaraProgram_of_sexp sexp_1 in
-  let prog_2 = Interface.coq_CaracaraProgram_of_sexp sexp_2 in
+  let prog_1 = CrTypeIF.coq_CaracaraProgram_of_sexp sexp_1 in
+  let prog_2 = CrTypeIF.coq_CaracaraProgram_of_sexp sexp_2 in
   let res = SmtQuery.equivalence_checker_cr_dsl prog_1 prog_2 in
   match res with
   | Equivalent -> print_endline "Equivalent"
