extracted_code/MemEq.ml
@@ -1,0 +1,37 @@
+open Sexplib
+open CrTypeIF.CrMem
+
+let load f =
+  let x = open_in f in
+  let len = in_channel_length x in
+  let str = really_input_string x len in
+  close_in x;
+  str
+
+let () =
+  if Array.length Sys.argv != 3 then (
+    prerr_endline "usage: ./bin <file_a> <file_b>";
+    exit 1
+  );
+
+  let file_1 = Sys.argv.(1) in
+  let f1_str = load file_1 in
+  let file_2 = Sys.argv.(2) in
+  let f2_str = load file_2 in
+
+  let sexp1 = Sexp.of_string f1_str in
+  let sexp2 = Sexp.of_string f2_str in
+
+  let prog1 = coq_MemProgram_of_sexp sexp1 in
+  let prog2 = coq_MemProgram_of_sexp sexp2 in
+
+  let eq_query = CrMem.query_expression prog1 prog2 in
+
+  (* let eqq_s = sexp_of_coq_Z3Bool eq_query in
+  print_endline(Sexp.to_string_hum eqq_s); *)
+
+  let res = MemSolver.mem_solve eq_query in
+  match res with
+  | Z3Sat (_, _) -> print_endline("sat")
+  | Z3Unsat -> print_endline("unsat")
+  | Z3Unknown -> print_endline("unknown")
