extracted_code/Z3Solver.ml
@@ -9,6 +9,7 @@ end
 module StringMap = Stdlib.Map.Make(CoqStringOrd)
 type var_tracker = Z3.Expr.expr StringMap.t ref
 
+(*
 let rec z3_expr_from_coq_smt_bool_expr (expr : SmtExpr.coq_SmtBoolExpr) (ctx : Z3.context) (vars : var_tracker)
   : Z3.Expr.expr =
   match expr with
@@ -21,9 +22,9 @@ let rec z3_expr_from_coq_smt_bool_expr (expr : SmtExpr.coq_SmtBoolExpr) (ctx : Z
 and z3_expr_from_coq_smt_arith_expr (expr : SmtExpr.coq_SmtArithExpr) (ctx : Z3.context) (vars : var_tracker)
   : Z3.Expr.expr =
   match expr with
-  | SmtExpr.SmtConst n -> Z3.BitVector.mk_numeral ctx (string_of_int (Interface.coq_Z_to_int n)) 8
+  | SmtExpr.SmtConst n -> Z3.BitVector.mk_numeral ctx (string_of_int (CrTypeIF.coq_Z_to_int n)) 8
   | SmtExpr.SmtArithVar name -> (
-    let name_str = Interface.coq_str_to_str name in
+    let name_str = CrTypeIF.coq_str_to_str name in
     match StringMap.find_opt name_str !vars with
     | Some z3_var -> z3_var
     | None ->
@@ -41,18 +42,19 @@ and z3_expr_from_coq_smt_arith_expr (expr : SmtExpr.coq_SmtArithExpr) (ctx : Z3.
   | SmtExpr.SmtBitMul (e1, e2) -> Z3.BitVector.mk_mul ctx (z3_expr_from_coq_smt_arith_expr e1 ctx vars) (z3_expr_from_coq_smt_arith_expr e2 ctx vars)
   | SmtExpr.SmtBitDiv (e1, e2) -> Z3.BitVector.mk_udiv ctx (z3_expr_from_coq_smt_arith_expr e1 ctx vars) (z3_expr_from_coq_smt_arith_expr e2 ctx vars)
   | SmtExpr.SmtBitMod (e1, e2) -> Z3.BitVector.mk_smod ctx (z3_expr_from_coq_smt_arith_expr e1 ctx vars) (z3_expr_from_coq_smt_arith_expr e2 ctx vars)
+*)
 
 (* Gets all variable assignments and folds them into a valuation (linked list) *)
-let to_vmap (m : Z3.Model.model) (acc : Interface.coq_ValueMap) (name : string) (z3_var : Z3.Expr.expr) : Interface.coq_ValueMap =
+let to_vmap (m : Z3.Model.model) (acc : Shim.coq_ValueMap) (name : string) (z3_var : Z3.Expr.expr) : Shim.coq_ValueMap =
   match Z3.Model.eval m z3_var true with
   | Some v ->
     if Z3.Expr.is_numeral v then
       let var_str = Z3.BitVector.numeral_to_string v in
       let var_val = int_of_string var_str in
       Printf.printf "| var( \027[1m%s\027[0m ) := %d\n" name var_val;
-      Interface.VMap (
-        Interface.str_to_coq_str name,
-        Interface.int_to_coq_uint8 var_val,
+      Shim.VMap (
+        Shim.str_to_coq_str name,
+        Shim.int_to_coq_uint8 var_val,
         acc)
     else
       raise (Failure ("Expects uint8 but got non-numeral value for " ^ name))
@@ -70,13 +72,15 @@ let sat_check solver tracked_vars =
       let var_bindings = StringMap.bindings !tracked_vars in
       let valuations = Stdlib.List.fold_left
         (fun acc (name, z3_var) -> to_vmap m acc name z3_var)
-        Interface.VMap_DNE
+        Shim.VMap_DNE
         var_bindings in
       Printf.printf "└\n";
-      SmtTypes.SmtSat (Interface.coq_TraverseMap valuations))
+      SmtTypes.SmtSat (Shim.coq_TraverseMap valuations))
     | None -> raise (Failure "Z3 returned SAT, but no valuation."))
 
 let solve (expr : SmtExpr.coq_SmtBoolExpr) =
+  let _ = expr in
+  (*
   let ctx = mk_context [] in
   let solver = Solver.mk_solver ctx None in
   let tracked_vars = ref StringMap.empty in
@@ -84,3 +88,5 @@ let solve (expr : SmtExpr.coq_SmtBoolExpr) =
   Solver.add solver [z3_expr];
 
   sat_check solver tracked_vars
+  *)
+  SmtTypes.SmtUnknown
