CrMemEx.v
@@ -1,0 +1,85 @@
+From MyProject Require Import CrMem.
+From MyProject Require Import CrVal.
+From MyProject Require Import CrIdentifiers.
+From MyProject Require Import SmtExpr.
+From MyProject Require Import Maps.
+From MyProject Require Import Integers.
+From MyProject Require Import MyInts.
+Require Import ZArith.
+From Coq.Strings Require Import String.
+From Coq.Strings Require Import Ascii.
+Require Import List.
+Import ListNotations.
+
+
+Definition rdi : positive := 1.
+Definition rsi : positive := 2.
+Definition rdx : positive := 3.
+Definition rcx : positive := 4.
+Definition rax : positive := 5.
+
+Definition local_x := (TmpArg 1%positive).
+Definition b_plus_c := (TmpArg 2%positive).
+Definition x4_val := (TmpArg 3%positive).
+Definition two_plus_two := (TmpArg 4%positive).
+
+Definition p1 : MemProgram := {|
+  fn_in := [
+    (rdi, uintptr_t);
+    (rsi, uint8_t);
+    (rdx, uint8_t)
+  ];
+  fn_body := [
+    AllocOp local_x
+      (ValArg (imm_ptr (repr 0x400)))
+      (ValArg (imm_u32 (repr 16)));
+    AddOp b_plus_c
+      (IOArg rsi)
+      (IOArg rdx);
+    StOp local_x
+      (ValArg (imm_u32 (repr 4)))
+      b_plus_c;
+    LdOp x4_val
+      local_x
+      (ValArg (imm_u32 (repr 4)));
+    StOp (IOArg rdi)
+      (ValArg (imm_u32 (repr 0)))
+      x4_val
+  ];
+  fn_out_vars := [];
+  fn_out_iaddrs := [];
+  fn_out_vaddrs := [(rdi, (repr 0))];
+|}.
+
+Compute List.map (vptr_val (compile_sym p1)) (fn_out_vaddrs p1).
+
+Definition p2 : MemProgram := {|
+  fn_in := [
+    (rdi, uintptr_t);
+    (rsi, uint8_t);
+    (rdx, uint8_t)
+  ];
+  fn_body := [
+    AllocOp local_x
+      (ValArg (imm_ptr (repr 0x400)))
+      (ValArg (imm_u32 (repr 16)));
+    AddOp b_plus_c
+      (IOArg rsi)
+      (IOArg rdx);
+    AddOp two_plus_two
+      (ValArg (imm_u32 (repr 2)))
+      (ValArg (imm_u32 (repr 2)));
+    StOp local_x
+      (ValArg (imm_u32 (repr 4)))
+      b_plus_c;
+    LdOp x4_val
+      local_x
+      two_plus_two;
+    StOp (IOArg rdi)
+      (ValArg (imm_u32 (repr 0)))
+      x4_val
+  ];
+  fn_out_vars := [];
+  fn_out_iaddrs := [];
+  fn_out_vaddrs := [(rdi, (repr 0))];
+|}.
