Extraction.v
@@ -4,10 +4,15 @@ Extraction Language OCaml.
 From MyProject Require Import SmtQuery.
 From MyProject Require Import Integers.
 
+From MyProject Require Import CrVal.
+From MyProject Require Import CrMem.
+From MyProject Require Import CrMemEx.
+
 (* Tell extraction to use your external OCaml implementation *)
 Extract Constant smt_query => "Z3Solver.solve".
+Extract Constant z3_query => "MemSolver.mem_solve".
 
 Set Extraction Output Directory "extracted_code".
 
 (* Extract everything else normally *)
-Separate Extraction CrDsl.CaracaraProgram Integers.repr SmtQuery.equivalence_checker_cr_dsl SmtTypes.SmtResult.
+Separate Extraction CrMem.query_expression CrMem.Z3Res CrDsl.CaracaraProgram Integers.repr SmtQuery.equivalence_checker_cr_dsl SmtTypes.SmtResult.
